Proving elim_let alpha lemma
Proved that free vars satisfying alpha_equiv_var same in alpha terms
Wrote lemma for [elim_let], proved let assuming substitution
Proved (almost) safe_sub_t assuming sub_t
Proved var and let case of sub_t

src/proofs/ElimLet.v
@@ -239,6 +239,607 @@ Proof.
     eapply a_equiv_f_trans. apply Halphaf.  
     apply Alpha. *)
 
+Lemma alpha_equiv_var_sym m1 m2 x y:
+  alpha_equiv_var m1 m2 x y -> alpha_equiv_var m2 m1 y x.
+Proof.
+  rewrite !alpha_equiv_var_iff.
+  intros [[Hlook1 Hlook2] | [Hlook1 [Hlook2 Heq]]]; subst; auto.
+Qed.
+
+Lemma alpha_equiv_var_uniq m1 m2 x y z:
+  alpha_equiv_var m1 m2 x y ->
+  alpha_equiv_var m1 m2 x z ->
+  y = z.
+Proof.
+  rewrite !alpha_equiv_var_iff.
+  intros [[Hlook1 Hlook2] | [Hlook1 [Hlook2 Heq]]] [[Hlook3 Hlook4] | [Hlook3 [Hlook4 Heq2]]]; subst; auto;
+  rewrite Hlook1 in Hlook3; inversion Hlook3; auto.
+Qed.
+
+Lemma alpha_equiv_map_fv x y t1 f1:
+  (forall m1 m2 t2 (Hv: amap_lookup m1 x = Some y) (Halpha: alpha_equiv_t m1 m2 t1 t2),
+    aset_mem x (tm_fv t1) -> amap_lookup m2 y = Some x /\ aset_mem y (tm_fv t2)) /\
+  (forall m1 m2 f2 (Hv: amap_lookup m1 x = Some y) (Halpha: alpha_equiv_f m1 m2 f1 f2),
+    aset_mem x (fmla_fv f1) -> amap_lookup m2 y = Some x /\ aset_mem y (fmla_fv f2)).
+Proof.
+  revert t1 f1; apply term_formula_ind; simpl.
+  - intros c m1 m2 t2 Hv Halpha. destruct t2; try discriminate. 
+  - (*Tvar *)
+    intros v m1 m2 t2 Hv Halpha. destruct t2; try discriminate. simpl.
+    simpl_set. intros; subst.
+    rewrite alpha_equiv_var_iff in Halpha.
+    destruct Halpha as [[Hlook1 Hlook2] | [Hlook3 [Hlook4 Heq]]]; subst.
+    + rewrite Hlook1 in Hv; inversion Hv; subst; auto.
+    + rewrite Hlook3 in Hv; discriminate.
+  - (*Tfun*)
+    intros f1 tys1 tms1 IH m1 m2 t2 Hv Halpha. destruct t2 as [| | f2 tys2 tms2 | | | | ]; try discriminate.
+    simpl. destruct (funsym_eq_dec f1 f2); subst; [|discriminate]; simpl in Halpha. 
+    destruct (Nat.eqb_spec (length tms1) (length tms2)) as [Hlen|]; [|discriminate]; simpl in *.
+    destruct (list_eq_dec _ tys1 tys2); [|discriminate]; subst. simpl in *.
+    generalize dependent tms2. induction tms1 as [| t1 tms1 IHtms]; intros [| t2 tms2]; try discriminate; simpl; auto.
+    rewrite !all2_cons, !andb_true.
+    intros [Halpha Hall] Hlentms. inversion IH as [| ? ? IH1 IH2]; subst.
+    simpl_set_small. intros [Hmemx | Hmemx]; auto.
+    + apply IH1 in Halpha; auto. destruct_all; auto.
+    + specialize (IHtms IH2 _ Hall ltac:(lia) Hmemx). destruct_all; auto.
+  - (*Tlet - interesting*)
+    intros tm1 v1 tm2 IH1 IH2 m1 m2 t2 Hv Halpha.
+    destruct t2 as [| | | e1 v2 e3 | | | ]; try discriminate.
+    simpl. destruct (vty_eq_dec (snd v1) (snd v2)) as [Htyeq|]; [|discriminate]; simpl in Halpha.
+    rewrite andb_true in Halpha. destruct Halpha as [Halpha1 Halpha2].
+    simpl_set. intros [Hxfv | [Hxfv Hxv1]].
+    + apply IH1 in Halpha1; auto. destruct Halpha1 as [Hlook2 Hmemy]; auto.
+    + (*Why we need the [amap_lookup] condition: this proves that y <> v2*) apply IH2 in Halpha2; auto.
+      2: { rewrite amap_set_lookup_diff; auto. }
+      destruct Halpha2 as [Hlook2 Hmemy].
+      (*Here, know that y <> v2. Otherwise, v1 = x, a contradiction. This also proves the lookup condition*)
+      vsym_eq y v2.
+      1: { rewrite amap_set_lookup_same in Hlook2. inversion Hlook2; subst; contradiction. }
+      rewrite amap_set_lookup_diff in Hlook2; auto.
+  - (*Tif*)
+    intros f t1 t2 IH1 IH2 IH3 m1 m2 tm2 Hv Halpha.
+    destruct tm2; try discriminate.
+    simpl. simpl_set. rewrite !andb_true in Halpha.
+    destruct Halpha as [[Ha1 Ha2] Ha3].
+    intros [Hfv | [Hfv | Hfv]]; [apply IH1 in Ha1; auto| apply IH2 in Ha2; auto |apply IH3 in Ha3; auto];
+    destruct_all; auto.
+  - (*Tmatch*)
+    intros tm1 v1 ps1 IH1 IHps1 m1 m2 t2 Hv Halpha.
+    destruct t2 as [| | | | | tm2 v2 ps2 |]; try discriminate.
+    simpl. rewrite !andb_true in Halpha. destruct Halpha as [[[Halpha Hlenps] Hv12] Hall].
+    apply Nat.eqb_eq in Hlenps.
+    simpl_set_small. intros [Hfv | Hfv].
+    1 : { apply IH1 in Halpha; auto. destruct_all; auto. }
+    (*Get rid of "or"*)
+    assert (amap_lookup m2 y = Some x /\
+       aset_mem y
+         (aset_big_union (fun x0 : pattern * term => aset_diff (pat_fv (fst x0)) (tm_fv (snd x0))) ps2));
+    [| destruct_all; auto].
+    clear -IHps1 Hlenps Hall Hfv Hv.
+    generalize dependent ps2. induction ps1 as [| [p1 t1] ps1 IHps]; intros [| [p2 t2] ps2]; simpl; try discriminate; auto.
+    intros Hlenps. rewrite all2_cons. simpl.
+    destruct (a_equiv_p p1 p2) as [[r1 r2]|] eqn : Halphap; [|discriminate].
+    rewrite andb_true. intros [Halphat Hall]. simpl_set_small.
+    simpl in Hfv. inversion IHps1 as [|? ? IH1 IH2]; subst; clear IHps1. destruct Hfv as [Hmemx | Hmemx].
+    + (*head case*)
+      clear IH2 IHps Hall.
+      simpl_set_small. destruct Hmemx as [Hmemx Hnotfv].
+      (*Use properties of r1 and r2*)
+      assert (Ha:=Halphap). apply a_equiv_p_vars_iff in Ha. simpl in Ha. destruct Ha as [Ha1 Ha2].
+      apply IH1 in Halphat; auto.
+      2: { rewrite aunion_lookup. specialize (Ha1 x). rewrite amap_mem_spec in Ha1.
+        destruct (amap_lookup r1 x); auto.
+        exfalso. apply Hnotfv. apply Ha1. reflexivity.
+      }
+      destruct Halphat as [Hlook2 Hmemy].
+      rewrite aunion_lookup in Hlook2.
+      destruct (amap_lookup r2 y) eqn : Hr2.
+      * inversion Hlook2; subst; clear Hlook2.
+        (*So now we know that r1(x) = y - but then x is in pat_fv p1, contradiction*)
+        apply a_equiv_p_bij in Halphap. simpl in Halphap. unfold bij_map in Halphap.
+        apply Halphap in Hr2. exfalso. apply Hnotfv. apply Ha1. rewrite amap_mem_spec, Hr2. reflexivity.
+      * (*In this case, know that y not in [pat_fv p2], bc not in r2*)
+        split; auto. left. split; auto. intros Hyfv.
+        apply Ha2 in Hyfv. rewrite amap_mem_spec, Hr2 in Hyfv. discriminate.
+    + (*IH case*)
+      specialize (IHps IH2 Hmemx ps2 ltac:(lia) Hall).
+      destruct_all; auto.
+  - (*Teps*)
+    intros f1 v1 IH m1 m2 t2 Hv Halpha. destruct t2 as [| | | | | | f2 v2]; try discriminate.
+    simpl. rewrite andb_true in Halpha. destruct Halpha as [Hty Halpha].
+    simpl_set. intros [Hxfv Hxv1].
+    apply IH in Halpha; auto.
+    2: { rewrite amap_set_lookup_diff; auto. }
+    destruct Halpha as [Hlook2 Hmemy].
+    vsym_eq y v2.
+    + rewrite amap_set_lookup_same in Hlook2. inversion Hlook2; subst; contradiction.
+    + rewrite amap_set_lookup_diff in Hlook2; auto.
+  - (*Fpred*)
+    intros p1 tys1 tms1 IH m1 m2 t2 Hv Halpha. destruct t2 as [p2 tys2 tms2 | | | | | | | | |]; try discriminate.
+    simpl. destruct (predsym_eq_dec p1 p2); subst; [|discriminate]; simpl in Halpha. 
+    destruct (Nat.eqb_spec (length tms1) (length tms2)) as [Hlen|]; [|discriminate]; simpl in *.
+    destruct (list_eq_dec _ tys1 tys2); [|discriminate]; subst. simpl in *.
+    generalize dependent tms2. induction tms1 as [| t1 tms1 IHtms]; intros [| t2 tms2]; try discriminate; simpl; auto.
+    rewrite !all2_cons, !andb_true.
+    intros [Halpha Hall] Hlentms. inversion IH as [| ? ? IH1 IH2]; subst.
+    simpl_set_small. intros [Hmemx | Hmemx]; auto.
+    + apply IH1 in Halpha; auto. destruct_all; auto.
+    + specialize (IHtms IH2 _ Hall ltac:(lia) Hmemx). destruct_all; auto.
+  - (*Fquant*)
+    intros q1 v1 f1 IH m1 m2 f2 Hv Halpha.
+    destruct f2 as [| q2 v2 f2 | | | | | | | |]; try discriminate.
+    simpl. rewrite !andb_true in Halpha. destruct Halpha as [_ Halpha].
+    simpl_set. intros [Hxfv Hxv1].
+    apply IH in Halpha; auto.
+    2: { rewrite amap_set_lookup_diff; auto. }
+    destruct Halpha as [Hlook2 Hmemy].
+    vsym_eq y v2.
+    + rewrite amap_set_lookup_same in Hlook2. inversion Hlook2; subst; contradiction.
+    + rewrite amap_set_lookup_diff in Hlook2; auto.
+  - (*Feq*)
+    intros ty t1 t2 IH1 IH2 m1 m2 f2 Hv Halpha.
+    destruct f2; try discriminate.
+    simpl. simpl_set. rewrite !andb_true in Halpha.
+    destruct Halpha as [[_ Ha1] Ha2].
+    intros [Hfv | Hfv]; [apply IH1 in Ha1; auto| apply IH2 in Ha2; auto];
+    destruct_all; auto.
+  - (*Fbinop*)
+    intros b f1 f2 IH1 IH2 m1 m2 fm2 Hv Halpha.
+    destruct fm2; try discriminate.
+    simpl. simpl_set. rewrite !andb_true in Halpha.
+    destruct Halpha as [[_ Ha1] Ha2].
+    intros [Hfv | Hfv]; [apply IH1 in Ha1; auto| apply IH2 in Ha2; auto];
+    destruct_all; auto.
+  - (*Fnot*)
+    intros f1 IH m1 m2 f2 Hv Halpha. destruct f2; try discriminate.
+    intros Hfv.
+    apply IH in Halpha; auto.
+  - (*Ftrue*) intros m1 m2 f2 Hv Halpha. destruct f2; try discriminate; auto.
+  - (*Ffalse*) intros m1 m2 f2 Hv Halpha. destruct f2; try discriminate; auto.
+  - (*Flet*) 
+    intros tm1 v1 tm2 IH1 IH2 m1 m2 t2 Hv Halpha.
+    destruct t2 as [| | | | | | | e1 v2 e3 | | ]; try discriminate.
+    simpl. destruct (vty_eq_dec (snd v1) (snd v2)) as [Htyeq|]; [|discriminate]; simpl in Halpha.
+    rewrite andb_true in Halpha. destruct Halpha as [Halpha1 Halpha2].
+    simpl_set. intros [Hxfv | [Hxfv Hxv1]].
+    + apply IH1 in Halpha1; auto. destruct Halpha1 as [Hlook2 Hmemy]; auto.
+    + apply IH2 in Halpha2; auto.
+      2: { rewrite amap_set_lookup_diff; auto. }
+      destruct Halpha2 as [Hlook2 Hmemy]. vsym_eq y v2.
+      * rewrite amap_set_lookup_same in Hlook2. inversion Hlook2; subst; contradiction.
+      * rewrite amap_set_lookup_diff in Hlook2; auto.
+  - (*Fif*)
+    intros f1 f2 f3 IH1 IH2 IH3 m1 m2 fm1 Hv Halpha.
+    destruct fm1; try discriminate.
+    simpl. simpl_set. rewrite !andb_true in Halpha.
+    destruct Halpha as [[Ha1 Ha2] Ha3].
+    intros [Hfv | [Hfv | Hfv]]; [apply IH1 in Ha1; auto| apply IH2 in Ha2; auto |apply IH3 in Ha3; auto];
+    destruct_all; auto.
+  - (*Fmatch*)
+    intros tm1 v1 ps1 IH1 IHps1 m1 m2 t2 Hv Halpha.
+    destruct t2 as [| | | | | | | | | tm2 v2 ps2]; try discriminate.
+    simpl. rewrite !andb_true in Halpha. destruct Halpha as [[[Halpha Hlenps] Hv12] Hall].
+    apply Nat.eqb_eq in Hlenps.
+    simpl_set_small. intros [Hfv | Hfv].
+    1 : { apply IH1 in Halpha; auto. destruct_all; auto. }
+    assert (amap_lookup m2 y = Some x /\
+       aset_mem y
+         (aset_big_union (fun x0 : pattern * formula => aset_diff (pat_fv (fst x0)) (fmla_fv (snd x0))) ps2));
+    [| destruct_all; auto].
+    clear -IHps1 Hlenps Hall Hfv Hv.
+    generalize dependent ps2. induction ps1 as [| [p1 t1] ps1 IHps]; intros [| [p2 t2] ps2]; simpl; try discriminate; auto.
+    intros Hlenps. rewrite all2_cons. simpl.
+    destruct (a_equiv_p p1 p2) as [[r1 r2]|] eqn : Halphap; [|discriminate].
+    rewrite andb_true. intros [Halphat Hall]. simpl_set_small.
+    simpl in Hfv. inversion IHps1 as [|? ? IH1 IH2]; subst; clear IHps1. destruct Hfv as [Hmemx | Hmemx].
+    + (*head case*)
+      clear IH2 IHps Hall.
+      simpl_set_small. destruct Hmemx as [Hmemx Hnotfv].
+      assert (Ha:=Halphap). apply a_equiv_p_vars_iff in Ha. simpl in Ha. destruct Ha as [Ha1 Ha2].
+      apply IH1 in Halphat; auto.
+      2: { rewrite aunion_lookup. specialize (Ha1 x). rewrite amap_mem_spec in Ha1.
+        destruct (amap_lookup r1 x); auto.
+        exfalso. apply Hnotfv. apply Ha1. reflexivity.
+      }
+      destruct Halphat as [Hlook2 Hmemy].
+      rewrite aunion_lookup in Hlook2.
+      destruct (amap_lookup r2 y) eqn : Hr2.
+      * inversion Hlook2; subst; clear Hlook2.
+        apply a_equiv_p_bij in Halphap. simpl in Halphap. unfold bij_map in Halphap.
+        apply Halphap in Hr2. exfalso. apply Hnotfv. apply Ha1. rewrite amap_mem_spec, Hr2. reflexivity.
+      * split; auto. left. split; auto. intros Hyfv.
+        apply Ha2 in Hyfv. rewrite amap_mem_spec, Hr2 in Hyfv. discriminate.
+    + (*IH case*)
+      specialize (IHps IH2 Hmemx ps2 ltac:(lia) Hall).
+      destruct_all; auto.
+Qed.
+
+Definition alpha_equiv_t_map_fv m1 m2 t1 t2 x y
+  (Halpha: alpha_equiv_t m1 m2 t1 t2)
+  (Hxy: amap_lookup m1 x = Some y)
+  (Hfv: aset_mem x (tm_fv t1)):
+  amap_lookup m2 y = Some x /\ aset_mem y (tm_fv t2) :=
+  proj_tm (alpha_equiv_map_fv x y) t1 m1 m2 t2 Hxy Halpha Hfv.
+
+Definition alpha_equiv_f_map_fv m1 m2 f1 f2 x y
+  (Halpha: alpha_equiv_f m1 m2 f1 f2)
+  (Hxy: amap_lookup m1 x = Some y)
+  (Hfv: aset_mem x (fmla_fv f1)):
+  amap_lookup m2 y = Some x /\ aset_mem y (fmla_fv f2) :=
+  proj_fmla (alpha_equiv_map_fv x y) f1 m1 m2 f2 Hxy Halpha Hfv.
+
+(*More useful corollaries*)
+(*First, an aux lemma*)
+Lemma alpha_equiv_t_map_fv_aux m1 m2 t1 t2 x y
+  (Halpha: alpha_equiv_t m1 m2 t1 t2)
+  (Hvar: alpha_equiv_var m1 m2 x y):
+  aset_mem x (tm_fv t1) -> aset_mem y (tm_fv t2).
+Proof.
+  rewrite alpha_equiv_var_iff in Hvar.
+  destruct Hvar as [[Hlook1 Hlook2] | [Hlook1 [Hlook2 Heq]]]; subst.
+  - intros Hfv. apply alpha_equiv_t_map_fv with(x:=x)(y:=y) in Halpha; auto.
+    destruct_all; auto.
+  - apply alpha_t_fv_filter in Halpha.
+    apply (f_equal (fun s => aset_mem y s)) in Halpha.
+    (*Why is it here? - provable half of propext*)
+    apply ZifyClasses.eq_iff in Halpha.
+    rewrite !aset_mem_filter in Halpha.
+    intros Hmem.
+    apply Halpha. split; auto.
+    rewrite amap_mem_spec, Hlook1. auto.
+Qed.
+
+(*Then the iff (what we wanted to prove)*)
+Corollary alpha_equiv_t_map_fv_iff m1 m2 t1 t2 x y
+  (Halpha: alpha_equiv_t m1 m2 t1 t2)
+  (Hvar: alpha_equiv_var m1 m2 x y):
+  aset_mem x (tm_fv t1) <-> aset_mem y (tm_fv t2).
+Proof.
+  split.
+  - eapply alpha_equiv_t_map_fv_aux; eauto.
+  - apply alpha_equiv_t_map_fv_aux with (m1:=m2)(m2:=m1).
+    + rewrite alpha_equiv_t_sym; auto.
+    + apply alpha_equiv_var_sym; auto.
+Qed.
+
+(*TODO: formula version*)
+
+(*General [same_in] - TODO: replace other version with this*)
+
+Fixpoint same_in_p (p1 p2: pattern) (x y: vsymbol) : bool :=
+  match p1, p2 with
+  | Pvar v1, Pvar v2 => eqb (vsymbol_eq_dec v1 x) (vsymbol_eq_dec v2 y)
+  | Pconstr f1 tys1 ps1, Pconstr t2 tys2 ps2 =>
+    (length ps1 =? length ps2) &&
+    all2 (fun p1 p2 => same_in_p p1 p2 x y) ps1 ps2
+  | Pwild, Pwild => true
+  | Por p1 p2, Por p3 p4 =>
+    same_in_p p1 p3 x y &&
+    same_in_p p2 p4 x y
+  | Pbind p1 v1, Pbind p2 v2 =>
+    same_in_p p1 p2 x y &&
+    eqb (vsymbol_eq_dec v1 x) (vsymbol_eq_dec v2 y)
+  | _, _ => false
+  end.
+
+Fixpoint same_in_t (t1 t2: term) (x y: vsymbol) : bool :=
+  match t1, t2 with
+  | Tconst _, Tconst _ => true
+  | Tvar v1, Tvar v2 => eqb (vsymbol_eq_dec v1 x) (vsymbol_eq_dec v2 y)
+  | Tlet tm1 v1 tm2, Tlet tm3 v2 tm4 =>
+    same_in_t tm1 tm3 x y &&
+    (eqb (vsymbol_eq_dec v1 x) (vsymbol_eq_dec v2 y)) &&
+    same_in_t tm2 tm4 x y
+  | Tfun f1 tys1 tms1, Tfun f2 tys2 tms2 =>
+    (length tms1 =? length tms2) &&
+    all2 (fun t1 t2 => same_in_t t1 t2 x y) tms1 tms2
+  | Tif f1 tm1 tm2, Tif f2 tm3 tm4 =>
+    same_in_f f1 f2 x y &&
+    same_in_t tm1 tm3 x y &&
+    same_in_t tm2 tm4 x y
+  | Tmatch tm1 v1 ps1, Tmatch tm2 v2 ps2 =>
+    (length ps1 =? length ps2) &&
+    same_in_t tm1 tm2 x y &&
+    all2 (fun x1 x2 => 
+      same_in_p (fst x1) (fst x2) x y &&
+      same_in_t (snd x1) (snd x2) x y) ps1 ps2
+  | Teps f1 v1, Teps f2 v2 =>
+    (eqb (vsymbol_eq_dec v1 x) (vsymbol_eq_dec v2 y)) &&
+    same_in_f f1 f2 x y
+  | _, _ => false
+  end
+with same_in_f (f1 f2: formula) (x y: vsymbol) : bool :=
+  match f1, f2 with
+  | Fpred p1 tys1 tms1, Fpred p2 tys2 tms2 =>
+    (length tms1 =? length tms2) &&
+    all2 (fun t1 t2 => same_in_t t1 t2 x y) tms1 tms2
+  | Fquant q1 v1 f1, Fquant q2 v2 f2 =>
+    eqb (vsymbol_eq_dec v1 x) (vsymbol_eq_dec v2 y) &&
+    same_in_f f1 f2 x y
+  | Feq v1 t1 t2, Feq v2 t3 t4 =>
+    same_in_t t1 t3 x y &&
+    same_in_t t2 t4 x y
+  | Fbinop b1 f1 f2, Fbinop b2 f3 f4 =>
+    same_in_f f1 f3 x y &&
+    same_in_f f2 f4 x y
+  | Fnot f1, Fnot f2 =>
+    same_in_f f1 f2 x y
+  | Ftrue, Ftrue => true
+  | Ffalse, Ffalse => true
+  | Flet tm1 v1 f1, Flet tm2 v2 f2 =>
+    same_in_t tm1 tm2 x y &&
+    (eqb (vsymbol_eq_dec v1 x) (vsymbol_eq_dec v2 y)) &&
+    same_in_f f1 f2 x y
+  | Fif f1 f2 f3, Fif f4 f5 f6 =>
+    same_in_f f1 f4 x y &&
+    same_in_f f2 f5 x y &&
+    same_in_f f3 f6 x y
+  | Fmatch tm1 v1 ps1, Fmatch tm2 v2 ps2 =>
+    (length ps1 =? length ps2) &&
+    same_in_t tm1 tm2 x y &&
+    all2 (fun x1 x2 => 
+     (* (length (pat_fv (fst x1)) =? length (pat_fv (fst x2))) && *)
+      same_in_p (fst x1) (fst x2) x y &&
+      same_in_f (snd x1) (snd x2) x y) ps1 ps2
+  | _, _ => false
+  end.
+
+Lemma keys_disj_equiv {A B: Type} `{countable.Countable A} (s: aset A) (m: amap A B):
+  (forall x, aset_mem x s -> amap_lookup m x = None) <-> aset_disj (keys m) s.
+Proof.
+  rewrite aset_disj_equiv.
+  split.
+  - intros Hnone x [Hx1 Hx2].
+    apply Hnone in Hx2. apply amap_lookup_none in Hx2. contradiction.
+  - intros Hdisj x Hmemx.
+    specialize (Hdisj x).
+    apply amap_lookup_none. tauto.
+Qed.
+
+Lemma aset_disj_union_l {A: Type} `{countable.Countable A} (s1 s2 s3: aset A):
+  aset_disj (aset_union s1 s2) s3 ->
+  aset_disj s1 s3.
+Proof.
+  apply disj_asubset2, union_asubset_l.
+Qed.
+
+Lemma aset_disj_union_r {A: Type} `{countable.Countable A} (s1 s2 s3: aset A):
+  aset_disj (aset_union s1 s2) s3 ->
+  aset_disj s2 s3.
+Proof.
+  apply disj_asubset2, union_asubset_r.
+Qed.
+
+Lemma aset_disj_singleton {A: Type} `{countable.Countable A} (x: A) (s: aset A):
+  aset_disj (aset_singleton x) s <-> ~ aset_mem x s.
+Proof.
+  rewrite aset_disj_equiv. split.
+  - intros Hnotin Hmemx.
+    specialize (Hnotin x). apply Hnotin; simpl_set; auto.
+  - intros Hnotin y [Hmem Hmem']. simpl_set. subst. contradiction.
+Qed.
+
+
+(*If tm1 and tm2 are alpha equivalent by m3 and m4
+  and t1 and t2 are alpha equivalent by m1 and m2
+  and x and y occur in t1 and t2 the same
+  then t1[tm1/x] is alpha equivalent to t2[tm2/y] by (m1 U m3) and (m2 U m4) (I hope)*)
+(*Could do for multiple sub, but dont need here*)
+Lemma alpha_equiv_sub tm1 tm2  x y t1 f1:
+  (forall t2 m1 m2 (Halpha2: alpha_equiv_t m1 m2 tm1 tm2) 
+    (Halpha1: alpha_equiv_t (amap_set m1 x y) (amap_set m2 y x) t1 t2) (Hsame: same_in_t t1 t2 x y)
+    (*avoid capture*) 
+    (Hdisj1: aset_disj (list_to_aset (tm_bnd t1)) (tm_fv tm1))
+    (Hdisj2: aset_disj (list_to_aset (tm_bnd t2)) (tm_fv tm2))
+    (*NOTE maybe cant assume this*)
+    (* (Hnofv1: forall x, aset_mem x (tm_fv tm1) -> amap_lookup m1 x = None)
+    (Hnofv2: forall x, aset_mem x (tm_fv tm2) -> amap_lookup m2 x = None) *),
+    (*TODO: do we need any further restrictions*)
+    alpha_equiv_t m1 m2 (sub_t tm1 x t1) (sub_t tm2 y t2)) /\
+  (forall f2 m1 m2 (Halpha2: alpha_equiv_t m1 m2 tm1 tm2)  
+    (Halpha1: alpha_equiv_f (amap_set m1 x y) (amap_set m2 y x) f1 f2) (Hsame: same_in_f f1 f2 x y)
+    (*avoid capture*) 
+    (Hdisj1: aset_disj (list_to_aset (fmla_bnd f1)) (tm_fv tm1))
+    (Hdisj2: aset_disj (list_to_aset (fmla_bnd f2)) (tm_fv tm2))
+    (* (Hnofv1: forall x, aset_mem x (tm_fv tm1) -> amap_lookup m1 x = None)
+    (Hnofv2: forall x, aset_mem x (tm_fv tm2) -> amap_lookup m2 x = None) *),
+    (*TODO: do we need any further restrictions*)
+    alpha_equiv_f m1 m2 (sub_f tm1 x f1) (sub_f tm2 y f2)).
+Proof.
+  revert t1 f1. apply term_formula_ind; simpl. (*TODO: try to do var and let case*)
+  - intros c t2 m1 m2 Halpha2 Halpha Hsame Hd1 Hd2.
+    destruct t2; try discriminate. simpl. auto.
+  - (*Tvar*)
+    intros v1 t2 m1 m2 Halpha2 Halpha Hsame Hd1 Hd2.
+    destruct t2 as [| v2 | | | | |]; try discriminate.
+    simpl. vsym_eq x v1.
+    + vsym_eq v1 v1. simpl in Hsame. vsym_eq v2 y. vsym_eq y y.
+    + vsym_eq v1 x. simpl in Hsame. vsym_eq v2 y. vsym_eq y v2.
+      simpl. (*Now prove from [amap_set]*)
+      rewrite !alpha_equiv_var_iff in Halpha |- *.
+      rewrite !amap_set_lookup_diff in Halpha; auto.
+  - admit.
+  - (*Tlet*)
+    intros e1 v1 e2 IH1 IH2 t2 m1 m2 Halpha2 Halpha Hsame Hd1 Hd2.
+    destruct t2 as [| | | e3 v2 e4 | | |]; try discriminate.
+    simpl.
+    simpl in Hd2.
+    rewrite !andb_true in Halpha.
+    destruct Halpha as [[Hty Ha1] Ha2].
+    rewrite !andb_true in Hsame. destruct Hsame as [[Hsame1 Heqvar] Hsame2].
+    rewrite !list_to_aset_cons, !list_to_aset_app in Hd1, Hd2.
+    apply IH1 in Ha1; auto.
+    2: { apply aset_disj_union_r, aset_disj_union_l in Hd1. auto. }
+    2: { apply aset_disj_union_r, aset_disj_union_l in Hd2. auto. }
+    vsym_eq v1 x.
+    + (*use same - crucial*)
+      simpl in Heqvar. vsym_eq x x. vsym_eq v2 y. vsym_eq y y.
+      rewrite !andb_true; split_all; auto.
+      (*Just setting x and y twice - same*)
+      rewrite !amap_set_twice in Ha2. auto.
+    + simpl in Heqvar. vsym_eq x v1. vsym_eq v2 y. vsym_eq y v2.
+      (*Here, nothing is equal - we can reorder*)
+      rewrite !andb_true; split_all; auto.
+      rewrite amap_set_reorder in Ha2; auto.
+      rewrite (amap_set_reorder _ y v2) in Ha2; auto.
+      apply IH2 in Ha2; auto.
+      2: { apply aset_disj_union_r, aset_disj_union_r in Hd1. auto. }
+      2: { apply aset_disj_union_r, aset_disj_union_r in Hd2. auto. }
+      (*Now we can remove these vars because not free*)
+      assert (Hv1: ~ aset_mem v1 (tm_fv tm1)).
+      { apply aset_disj_union_l in Hd1. apply aset_disj_singleton; auto. }
+      assert (Hv2: ~ aset_mem v2 (tm_fv tm2)).
+      { apply aset_disj_union_l in Hd2. apply aset_disj_singleton; auto. }
+      (*separate lemma?*)
+      rewrite <- alpha_equiv_t_remove with (y2:=v2) in Halpha2 |- *; auto.
+      rewrite amap_remove_set_same.
+      (*And remove the other side*)
+      rewrite alpha_equiv_t_sym in Halpha2 |- *.
+      rewrite <- alpha_equiv_t_remove with (y2:=v1) in Halpha2 |- *; auto.
+      rewrite amap_remove_set_same.
+      apply Halpha2.
+  - 
+Admitted.
+
+(*TODO: prove rest of cases but should be doable*)
+
+
+(*TODO: need type equality?*)
+Lemma safe_sub_t_alpha m1 m2 v1 v2 t1 t2 t3 t4
+  (Halpha1: alpha_equiv_t m1 m2 t1 t2)
+  (Halpha2: alpha_equiv_t (amap_set m1 v1 v2) (amap_set m2 v2 v1) t3 t4):
+  alpha_equiv_t m1 m2 (safe_sub_t t1 v1 t3) (safe_sub_t t2 v2 t4).
+Proof.
+  unfold safe_sub_t.
+  (*Why we needed the previous: v1 in fv of t3 iff v2 in fv of t4*)
+  assert (Hfvs: aset_mem v1 (tm_fv t3) <-> aset_mem v2 (tm_fv t4)). {
+    eapply alpha_equiv_t_map_fv_iff; eauto.
+    rewrite alpha_equiv_var_iff. rewrite !amap_set_lookup_same. auto.
+  }
+  (*Annoyingly, have to destruct by cases*)
+  destruct (aset_mem_dec v1 (tm_fv t3)) as [Hv1 | Hv1]; 
+  destruct (aset_mem_dec v2 (tm_fv t4)) as [Hv2 | Hv2]; [| tauto | tauto |].
+  2: {
+    (*In this case, can remove these from the map because free vars not present*)
+    rewrite <- alpha_equiv_t_remove with (y2:=v2) in Halpha2 |- *; auto.
+    rewrite amap_remove_set_same in Halpha2.
+    (*And remove the other side*)
+    rewrite alpha_equiv_t_sym in Halpha2 |- *.
+    rewrite <- alpha_equiv_t_remove with (y2:=v1) in Halpha2 |- *; auto.
+    rewrite amap_remove_set_same in Halpha2.
+    apply Halpha2.
+  }
+  (*It doesn't actually matter which we substitute. But the result is alpha equivalent to t3*)
+  set (t3':=(if existsb (fun x : vsymbol => in_bool vsymbol_eq_dec x (tm_bnd t3)) (aset_to_list (tm_fv t1))
+      then a_convert_t t3 (tm_fv t1)
+      else t3)).
+  set (t4':=(if existsb (fun x : vsymbol => in_bool vsymbol_eq_dec x (tm_bnd t4)) (aset_to_list (tm_fv t2))
+      then a_convert_t t4 (tm_fv t2)
+      else t4)).
+  assert (Ht3: a_equiv_t t3 t3'). {
+    unfold t3'. destruct (existsb _). 
+    - apply a_convert_t_equiv.
+    - apply a_equiv_t_refl.
+  }
+  assert (Ht4: a_equiv_t t4 t4'). {
+    unfold t4'. clear. destruct (existsb _). 
+    - apply a_convert_t_equiv.
+    - apply a_equiv_t_refl.
+  }
+  assert (Ht34: alpha_equiv_t (amap_set m1 v1 v2) (amap_set m2 v2 v1) t3' t4'). {
+    pose proof (alpha_equiv_t_trans t3' t3 t4' amap_empty amap_empty (amap_set m1 v1 v2) (amap_set m2 v2 v1)) as Htrans.
+    forward Htrans.
+    { rewrite alpha_equiv_t_sym; auto. }
+    forward Htrans.
+    { pose proof (alpha_equiv_t_trans t3 t4 t4' (amap_set m1 v1 v2) (amap_set m2 v2 v1) amap_empty amap_empty Halpha2 Ht4) 
+      as Htrans1.
+      rewrite alpha_comp_empty_r, alpha_comp_empty_l in Htrans1. auto.
+    }
+    rewrite alpha_comp_empty_r, alpha_comp_empty_l in Htrans. auto.
+  }
+  (*Should be provable with previous*)
+Admitted.
+
+
+
+(* alpha_equiv_sub_var_t_full:
+  forall (t t2 : term) (x y : vsymbol) (m1 m2 : amap vsymbol vsymbol),
+  snd x = snd y ->
+  ~ In y (tm_bnd t2) ->
+  ~ aset_mem y (tm_fv t2) ->
+  same_in_t t t2 x ->
+  ~ amap_mem y m2 ->
+  alpha_equiv_t m1 m2 t t2 -> alpha_equiv_t (amap_set m1 x y) (amap_set m2 y x) t (sub_var_t x y t2)
+ *)
+
+(*TODO: generalize, define previous by this*)
+
+
+
+
+Lemma elim_let_alpha_equiv b1 b2 t1 f1:
+  (forall m1 m2 t2 (Halpha: alpha_equiv_t m1 m2 t1 t2), 
+    alpha_equiv_t m1 m2 (elim_let_t b1 b2 t1) (elim_let_t b1 b2 t2)) /\
+  (forall m1 m2 f2 (Halpha: alpha_equiv_f m1 m2 f1 f2), 
+    alpha_equiv_f m1 m2 (elim_let_f b1 b2 f1) (elim_let_f b1 b2 f2)).
+Proof.
+  revert t1 f1; apply term_formula_ind; simpl.
+  - intros c _ _ t2 Halpha. destruct t2; try discriminate. simpl. auto.
+  - intros v m1 m2 t2 Halpha. destruct t2; try discriminate. simpl. auto.
+  - (*Tfun*)
+    intros f1 tys1 tms1 IH m1 m2 t2 Halpha. destruct t2 as [| | f2 tys2 tms2 | | | | ]; try discriminate.
+    simpl. destruct (funsym_eq_dec f1 f2); subst; [|discriminate]; simpl in Halpha. simpl.
+    rewrite !length_map. destruct (Nat.eqb_spec (length tms1) (length tms2)) as [Hlen|]; [|discriminate]; simpl in *.
+    destruct (list_eq_dec _ tys1 tys2); [|discriminate]; subst. simpl in *.
+    rewrite !all2_map.
+    generalize dependent tms2. induction tms1 as [| t1 tms1 IHtms]; intros [| t2 tms2]; try discriminate; simpl; auto.
+    rewrite !all2_cons, !andb_true.
+    intros [Halpha Hall] Hlentms. inversion IH as [| ? ? IH1 IH2]; subst.
+    split; auto.
+  - (*Tlet - interesting case*)
+    intros tm1 v1 tm2 IH1 IH2 m1 m2 t2 Halpha. destruct t2 as [| | | e1 v2 e3 | | | ]; try discriminate.
+    destruct (vty_eq_dec (snd v1) (snd v2)) as [Htyeq|]; [|discriminate]; simpl in Halpha.
+    rewrite andb_true in Halpha. destruct Halpha as [Halpha1 Halpha2].
+    destruct b1; simpl; auto.
+    2: { rewrite Htyeq. destruct (vty_eq_dec _ _); simpl; auto. rewrite andb_true; split; auto. }
+    apply IH1 in Halpha1.
+    apply IH2 in Halpha2.
+    set (t1 := (elim_let_t true b2 tm1) ) in *.
+    set (t2:=(elim_let_t true b2 e1)) in *.
+    set (t3:=(elim_let_t true b2 tm2)) in *.
+    set (t4:=(elim_let_t true b2 e3)) in *.
+    (*Could assume: tm1 and tm2 with m3 and m4, then t1 and t2 with m1 U m3 and m2 U m4
+      then want to show safe_sub_t with  *)
+    apply safe_sub_t_alpha; auto.
+Admitted.
+
+
+    Search elim_let_t tm_fv.
+
+
+
+    unfold safe_sub_t.
+    (*TODO: should do [safe_sub_t] in different lemma*)
+    (*oh btw I already have the free var optimization but only in [safe_sub_t]*)
+
+    Search alpha_equiv_t safe_sub_t.
+ 
+
+    Search all2 combine.
+    Search all2 "impl".
+
+
+
+
+all2_Forall2
+    Search all2 Forall2.
+
+
+ auto.
+    Search all2 map.
+
+
+    rewrite !map_length.
 
 (*The main part: prove related*)
 Theorem elim_let_related (tsk1 : TaskDefs.task) (tsk2 : Task.task):
@@ -298,6 +899,10 @@ Proof.
       (*TODO: prove these equal in separate lemmas for [change_*] lemmas since we change goal *)
       admit.
     - unfold a_equiv_task. simpl_task. bool_to_prop; split_all; auto.
+
+
+
+
       (*TODO: prove that a_equiv_f preserved by elim_let_f*)
       admit.
   }
